examples/schorr.v
@@ -22,7 +22,7 @@ From htt Require Import options model heapauto graph.
 (* helper lemmas *)
 (*****************)
 
-Lemma eq_connect_aux (g1 g2 : pregraph) p:
+Lemma eq_connect_aux A (g1 g2 : pregraph A) p:
         valid (g1 \+ g2) ->
         {subset dom g2 <= predC p} ->
         um_filterk p (g1 \+ g2) = um_filterk p g1.
@@ -31,7 +31,7 @@ move=>V /(umfiltk_subdom0 p (validR V)) S.
 by rewrite umfiltUn // S unitR. 
 Qed.
 
-Lemma connectUn_eq (g g1 g2 : pregraph) (p : pred node) x :
+Lemma connectUn_eq A (g g1 g2 : pregraph A) (p : pred node) x :
         valid (g \+ g1) ->
         valid (g \+ g2) ->
         {subset dom g1 <= p} ->
@@ -45,105 +45,411 @@ rewrite -[RHS]connect_umfiltk eq_connect_aux //.
 by move=>y /S2; rewrite !inE negbK.
 Qed.
 
+(*****************)
+(* Binary graphs *)
+(*****************)
+
+(* short notation for left/right node of x *)
+Notation lft g x := (get_nth g x 0).
+Notation rgh g x := (get_nth g x 1).
+
+Definition contents {A} (g : pregraph A) : nmap A := mapv fst g.
+
+HB.instance Definition _ A := 
+  OmapFun.copy (@contents A) (@contents A).
+
+Lemma In_contentsX A (g : pregraph A) x v :
+        (x, v) \In contents g <-> 
+        exists lks, (x, (v, lks)) \In g.
+Proof.
+rewrite In_omfX; split; last by case=>lks H; exists (v, lks).
+by case; case=>w lks /= H [<-{v}]; exists lks.
+Qed.
+
+Lemma In_contents A (g : pregraph A) x v lks :
+        (x, (v, lks)) \In g ->
+        (x, v) \In contents g.
+Proof. by rewrite In_contentsX; exists lks. Qed.
+
+Definition links {A} (g : pregraph A) : nmap (seq node) := mapv snd g.
+
+HB.instance Definition _ A := 
+  OmapFun.copy (@links A) (@links A).
+
+Lemma In_linksX A (g : pregraph A) x lks : 
+        (x, lks) \In links g <->
+        exists v, (x, (v, lks)) \In g.
+Proof.
+rewrite In_omfX; split; last by case=>v H; exists (v, lks).
+by case; case=>v lks' /= H [<-{lks}]; exists v.
+Qed.
+
+Lemma In_links A (g : pregraph A) x v lks : 
+        (x, (v, lks)) \In g ->
+        (x, lks) \In links g.
+Proof. by rewrite In_linksX; exists v. Qed.
+
+(* laying binary pregraph onto heap *)
+Definition lay2_k {A} (v : A * seq node) : dynamic id :=
+  idyn (v.1, (nth null v.2 0, nth null v.2 1)).
+Definition lay2 {A} (g : pregraph A) : heap := mapv lay2_k g.
+
+HB.instance Definition _ A := 
+  OmapFun.copy (@lay2 A) (@lay2 A).
+
+
+Canonical heap_PredType : PredType (nat * dynamic id) := 
+  um_PredType heap.
+Coercion Pred_of_nmap (x : heap) : {Pred _} := 
+  [eta Mem_UmMap x].
+
+Lemma In_layX A (g : pregraph A) x (v : A) lft rgh : 
+        (x, idyn (v, (lft, rgh))) \In lay2 g <->
+        exists lks, 
+          [/\ lft = nth null lks 0, 
+              rgh = nth null lks 1 & 
+              (x, (v, lks)) \In g].
+Proof.
+rewrite In_omfX; split; last first.
+- by case=>lks [->-> H]; exists (v, lks).
+case=>-[w lks] H /Some_inj/inj_pair2 /= [<-{v} <-<-].
+by exists lks.
+Qed.
+
+Lemma In_lay A (g : pregraph A) x (v : A) lks :
+        (x, (v, lks)) \In g ->
+        (x, idyn (v, (nth null lks 0, nth null lks 1))) \In lay2 g.
+Proof. by rewrite In_layX=>H; exists lks. Qed.
+
+Lemma In_lay2X A (g : pregraph A) x (v : A) lft rgh : 
+        n_pregraph_axiom 2 g ->
+        (x, idyn (v, (lft, rgh))) \In lay2 g <->
+        (x, (v, [:: lft; rgh])) \In g.
+Proof.
+move=>H; split; last first.
+- by move=>X; apply/In_layX; exists [:: lft; rgh].
+case/In_layX=>lks [L R X]. 
+rewrite -(_ : lks = [:: lft; rgh]) //.
+rewrite (In_graph X) (links_nth H (In_dom X)) /=.
+by rewrite /get_nth -(In_graph X) -L -R.
+Qed.
+
+Lemma In_lay2 A (g : pregraph A) x (v : A) lft rgh : 
+        n_pregraph_axiom 2 g ->
+        (x, (v, [:: lft; rgh])) \In g ->
+        (x, idyn (v, (lft, rgh))) \In lay2 g.
+Proof. by move=>H /In_lay2X-/(_ H). Qed.
+
+
+
+(* updating binary pregraph at node x *)
+
+(* pass v = None to just update links *)
+Definition bupd A (g : pregraph A) x (v : option A) (lft rgh : node) :=
+  if find x (contents g) is Some v' then 
+    if v is Some w then upd x (w, [:: lft; rgh]) g 
+    else upd x (v', [:: lft; rgh]) g
+  else undef.
+
+Lemma bupd_is_binary A (g : pregraph A) x v lft rgh : 
+        n_pregraph_axiom 2 g ->
+        n_pregraph_axiom 2 (@bupd A g x v lft rgh).
+Proof.
+move=>H z; rewrite /bupd find_omf /omfx /=.
+case: (find x g)=>[[m lnk]|//].
+case: v=>[w|]; rewrite domU inE /graph.links findU;
+case: (x =P 0)=>//= /eqP Nx; case: (z =P x)=>[_ V|_ Dz].
+- by rewrite V.
+- by rewrite H.
+- by rewrite V.
+by rewrite H.
+Qed.
+
+(* updating just contents *)
+Notation updC g x v := (bupd g x (Some v) (lft g x) (rgh g x)).
+(* updating just left link *)
+Notation updL g x l := (bupd g x (contents g x) l (rgh g x)).
+(* updating just right link *)
+Notation updR g x r := (bupd g x (contents g x) (lft g x) r).
+(* updating just contents and left link *)
+Notation updCL g x v l := (bupd g x (Some v) l (rgh g x)).
+(* updating just contents and right link *)
+Notation updCR g x v r := (bupd g x (Some v) (lft g x) r).
+
+Lemma glE A (g : pregraph A) (x : node) : 
+        n_pregraph_axiom 2 g ->
+        x \in dom g ->
+        graph.links g x = [:: lft g x; rgh g x].
+Proof. by move=>H D; rewrite (links_nth H D). Qed.
+
+Lemma glD A (g : pregraph A) (x : node) : 
+        n_pregraph_axiom 2 g ->
+        x \in dom g ->
+        (x, [:: lft g x; rgh g x]) \In links g.
+Proof.
+move=>H /[dup]/In_graphX R /(glE H) <-.
+by apply/In_linksX.
+Qed.
+
+Lemma getU A (g : pregraph A) (x : node) v lf rg i : 
+        get_nth (bupd g x v lf rg) x i = 
+        if x \notin dom g then null
+        else nth null [:: lf; rg] i.
+Proof.
+rewrite /get_nth/graph.links/bupd find_omf/omfx /=.
+case: (dom_find x)=>[|w /In_find H _]; first by rewrite nth_nil.
+by case: v=>[v|] /=; rewrite findU eqxx /= (In_cond H) (In_valid H).
+Qed.
+
 (****************)
 (* Schorr-Waite *)
 (****************)
 
-(* short notation for left/right child of x *)
-Notation gl g x := (get_nth g x 0).
-Notation gr g x := (get_nth g x 1).
-
 (* type of markings *)
-Inductive mark := L | R | LR.
+Inductive mark := U | L | R | LR.
 (* decidable equality on marks *)
 Definition eq_mark l1 l2 : bool :=
-  if (l1, l2) is ((L, L)|(R, R)|(LR, LR)) then true else false.
+  if (l1, l2) is ((U,U)|(L, L)|(R, R)|(LR, LR)) then true else false.
 Lemma eq_markP : Equality.axiom eq_mark.
 Proof. by case; case=>//=; constructor. Qed.
 HB.instance Definition _ := hasDecEq.Build mark eq_markP.
+
+Notation pregraph := (pregraph mark).
+
+Definition marked (g : pregraph) : pregraph := 
+  um_filterv (fun v => v.1 != U) g.
+HB.instance Definition _ := OmapFun.copy marked marked.
+
 
 (* marking of children *)
 
 (* given marking map m, x is m-child of y iff: *)
 (* - m y = L and x is left child of y *)
 (* - m y = R and x is right child of y *)
-Definition ch (m : nmap mark) (g : pregraph) (x y : nat) := 
-  [|| (find y m == Some L) && (gl g y == x) |
-      (find y m == Some R) && (gr g y == x)].
+Definition ch (g : pregraph) (x y : nat) := 
+  [|| (find y (contents g) == Some L) && (lft g y == x) |
+      (find y (contents g) == Some R) && (rgh g y == x)].
 
-Lemma chP (m : nmap mark) g x y : 
-        reflect [\/ (y, L) \In m /\ gl g y = x |
-                    (y, R) \In m /\ gr g y = x]
-                (ch m g x y).
+Lemma chP (g : pregraph) x y : 
+        reflect [\/ (y, L) \In contents g /\ lft g y = x |
+                    (y, R) \In contents g /\ rgh g y = x]
+                (ch g x y).
 Proof.
 rewrite /ch; case: orP=>H; constructor.
 - by case: H=>H; [left|right]; case/andP: H=>/eqP/In_find H /eqP.
 by case=>[][/In_find/eqP M /eqP G]; apply: H; [left|right]; apply/andP.
 Qed.
 
-Lemma chN0 m g x y :
-        ch m g x y ->
+Lemma chN0 g x y :
+        ch g x y ->
         y != null.
 Proof. by case/chP=>[][/In_dom/dom_cond]. Qed.
 
-Lemma ch_fun m g a b x :
-        ch m g a x ->
-        ch m g b x ->
+Lemma ch_fun g a b x :
+        ch g a x ->
+        ch g b x ->
         a = b.
 Proof. by case/chP=>[][H <-] /chP [][/(In_fun H) {}H <-]. Qed.
 
-Lemma ch_path m g s x :
+Lemma ch_path g s x :
         x \in s -> 
-        path (ch m g) null s -> 
-        exists y, y \in belast null s /\ ch m g y x.
+        path (ch g) null s -> 
+        exists y, y \in belast null s /\ ch g y x.
 Proof. exact: path_prev. Qed.
 
-Lemma ch_path_uniq m g s :
-        path (ch m g) null s -> 
+Lemma ch_path_uniq g s :
+        path (ch g) null s -> 
         uniq (null :: s).
 Proof. by apply: path_uniq; [apply: chN0|apply: ch_fun]. Qed.
 
-Definition upd_edge (m : nmap mark) g x y : seq node := 
-  if find x m is Some L then [:: y; gr g x] else [:: gl g x; y].
 
-Fixpoint rev_graph' m g ps t : pregraph := 
+Definition upd_edge g x y : mark * seq node := 
+  match find x (contents g) with
+  | Some L => (L, [:: y; rgh g x])
+  | _ => (R, [:: lft g x; y])
+  end.
+
+Fixpoint rev_graph' (g : pregraph) (ps : seq node) t : pregraph := 
   if ps is p :: ps then 
-    rev_graph' m (free g p) ps p \+ pts p (upd_edge m g p t)
+    rev_graph' (free g p) ps p \+ pts p (upd_edge g p t)
   else g.
 
-Definition rev_graph m g s t := rev_graph' m g (rev s) t.
+Definition rev_graph g s t := rev_graph' g (rev s) t.
 
 (* layout of graph+marking as heap *)
-Definition lay (m : nmap mark) (g : pregraph) : heap := 
+
+
+(*
+Definition lay (g : pregraph) : heap := 
   \big[join/Unit]_(x <- dom g) (x :-> (gl g x, gr g x, odflt L (find x m))).
 
-(* reach m g s t holds iff *)
+Lemma bigF (A : eqType) (xs : seq A) (f : A -> heap) k : 
+        valid (\big[join/Unit]_(i <- xs) f i) ->
+        free (\big[join/Unit]_(i <- xs) f i) k = 
+        \big[join/Unit]_(i <- xs) free (f i) k.
+Proof.
+elim: xs=>[|x xs IH].
+- by rewrite !big_nil free0.
+rewrite !big_cons => V.
+rewrite freeUn.
+case: ifP=>D.
+- rewrite IH //. rewrite (validR V). by [].
+rewrite -IH; last by rewrite (validX V).
+rewrite !freeND //.
+- apply: contraFN D=>D.
+  rewrite domUn inE D orbT andbT.
+  by [].
+apply: contraFN D=>D.
+by rewrite domUn inE (validX V) D.
+Qed.
+*)
+
+
+Lemma In_layE1 (g : pregraph) x pl pr c : 
+        n_pregraph_axiom 2 g ->
+        find x (lay2 g) = Some (idyn (c, (pl, pr))) ->
+        (x, (c, [:: pl; pr])) \In g.
+Proof. by move=>H /In_find /In_lay2X-/(_ H). Qed.
+
+Lemma In_layE2 (g : pregraph) x pl pr c : 
+        n_pregraph_axiom 2 g ->
+        (x, (c, [:: pl; pr])) \In g ->
+        find x (lay2 g) = Some (idyn (c, (pl, pr))).
+Proof. by move=>H /In_lay2X-/(_ H)/In_find. Qed.
+
+Lemma In_layX2 (g : pregraph) x c pl pr : 
+        n_pregraph_axiom 2 g ->
+        (x, (c, [:: pl; pr])) \In g ->
+        exists h, lay2 g = x :-> (c, (pl, pr)) \+ h.
+Proof. by move=>H Gx; eexists _; apply/heap_eta2/In_layE2. Qed.
+
+Lemma In_layX3 (g : pregraph) x l r c : 
+         lay2 (bupd g x (Some c) l r) = 
+         if x \in dom g then 
+           upd x (idyn (c, (l, r))) (lay2 g)
+         else undef.
+Proof.
+rewrite /lay2/bupd find_omf/omfx /=.
+case: (dom_find x)=>[|v]; first by rewrite omap_undef.
+move/In_find=>E _; rewrite (upd_eta x).
+rewrite omapPtUn -(upd_eta x) validU.
+rewrite (In_cond E) (In_valid E) /=.
+rewrite (upd_eta x) !omap_free !omap_omap.
+congr (_ \+ _); apply/eq_in_omap.
+by case=>k w /= H; case: (k =P x).
+Qed.
+
+Lemma In_layX4 (g : pregraph) x l r c : 
+         lay2 (x &-> (c, [:: l; r]) \+ g) = 
+         x :-> (c, (l, r)) \+ lay2 g.
+Proof.
+rewrite omfPtUn /=; case: ifP=>// V; set j := (_ \+ _).
+case: (normalP j)=>[->//|].
+rewrite !validPtUn valid_omap dom_omf_some // in V *.
+by rewrite V.
+Qed.
+
+(* reach g s t holds iff *)
 (* each unmarked node x in g is reachable through unmarked nodes *)
 (* - either starting from t, or *)
 (* - starting from a right child of some node in s *)
-Definition reach (m : nmap mark) (g : pregraph) (s : seq node) t := 
-  forall x, 
-    (* x is node in g *)
-    x \in dom g ->
-    (* x is unmarked *)
-    x \notin dom m ->
-    (* x is reachable from t avoiding marked nodes *)
-    (* Aleks note: if unmarked nodes are represented by a marking U *)
-    (* then this conjunct will have to change, as it currently assumes *)
-    (* that unmarked nodes are just those that aren't in m *)
-    x \in connect (mem (dom m)) g t \/
-    (* or x is reachable from some right child of a node y in s *)
-    (* avoiding marked nodes *)
-    exists y, y \in s /\ x \in connect (mem (dom m)) g (gr g y).
 
-Definition shape g0 r p t :=
-  fun h:heap =>  (exists s g m,
-              dom g  = dom h /\
-              h = lay m g /\ 
-              path (ch m g) null s /\ 
-              rev_graph m g s t = g0 /\
-              reach m g s t /\
-              {subset dom (um_filterv (predU (pred1 L) (pred1 LR)) m) <= s} /\ 
-              p = last null s /\
-              r = head t s /\
-              graph_axiom g).
+Definition reach (g : pregraph) (s : seq node) (t : node) := 
+  forall x, 
+    (* if x is unmarked node in g *)
+    (x, U) \In contents g ->
+    (* then x is reachable from t avoiding marked nodes *)
+    x \in connect (mem (dom (marked g))) g t \/
+    (* or x is reachable from some right child of a node in s *)
+    (* avoiding marked nodes *)
+    exists2 y, y \in s &
+      x \in connect (mem (dom (marked g))) g (rgh g y).
+
+UP TO HERE
+
+Definition shape (g0 g : pregraph) (m : nmap mark) (r p t : node) :=
+  fun h => exists stack, 
+    [/\ h = lay m g, 
+        {subset dom m <= dom g},
+        path (ch m g) null stack, 
+        rev_graph m g stack t = g0, 
+        reach m g stack t, 
+        {subset dom (um_filterv (predU (pred1 L) (pred1 LR)) m) <= stack},
+        p = last null stack, 
+        r = head t stack, 
+        n_pregraph_axiom 2 g &
+        graph_axiom g].
+
+Program Definition pop (p t : ptr): 
+  STsep {g0 g m r} (fun h => 
+    [/\ shape g0 g m r p t h,
+        (p, R) \In m &
+        t \in dom m \/ t = null],
+    [vfun res h => 
+       let: g' := upd p [:: gl g p; t] g in
+       let: m' := upd p LR m in
+         shape g0 g' m' r res.1 res.2 h /\
+         res = (gr g p, p)]) :=
+  Do (q <-- read (A:=node*node*mark) p;
+      p ::= (q.1.1, t, LR);;
+      ret (q.1.2, p)).
+Next Obligation.
+move=>p t [g0][g][m][r][/= h][H Pm D]. 
+case: H=>stack [-> H1 H2 H3 H4 H5 H6 H7 H8 H9].
+move: (H1 p (In_dom Pm))=>Pg.
+case/(glD H8)/(In_layX2 H8 H1): (Pg)=>h' E.
+rewrite E.
+do 3!step; split=>//; exists stack; split.
+- rewrite In_layX3.
+  - by rewrite upd_eta E freePtUn // (validX H).
+  - by rewrite (dom_valid Pg).
+  - by rewrite (In_valid Pm).
+  - by rewrite (In_cond Pm).
+
+Search upd.
+
+
+admit. 
+Admitted.
+
+Program Definition swing (p t : ptr):
+  STsep {g0 g m r} (fun h =>
+    [/\ shape g0 g m r p t h,
+        (p, L) \In m &
+        t \in dom m \/ t = null],
+    [vfun res h =>
+       let: g' := upd p [:: t; gl g p] g in
+       let: m' := upd p R m in
+         shape g0 g' m' r res.1 res.2 h /\
+         res = (t, gl g t) ]) :=
+  Do (q <-- read (A:=node*node*mark) p;
+      p ::= (t, q.1.1, R);;
+      ret (p, q.1.2)).
+Next Obligation.
+move=>p t [g0][g][m][r][/= h][H P D].
+case: H=>stack [-> H1 H2 H3 H4 H5 H6 H7 H8 H9].
+move: (H1 p (In_dom P))=>/(glD H8) /(In_layX2 H8 H1) [h' ->].
+do 3!step; split=>//. 
+exists stack; split =>//.
+admit.
+Admitted.
+
+Program Definition push (p t : ptr):
+  STsep {g0 g m r} (fun h =>
+    [/\ shape g0 g m r p t h,
+        t \in dom g &
+        t \notin dom m],
+    [vfun res h =>
+       let: g' := upd t [:: p; gr g t] g in
+       let: m' := upd t L m in
+         shape g0 g' m' r res.1 res.2 h /\
+         res = (t, gl g t) ]) :=
+  Do (q <-- read (A:=node*node*mark) t;
+      t ::= (p, q.1.2, L);;
+      ret (t, q.1.1)).
+Next Obligation.
+move=>p t [g0][g][m][r][/= h][H P D].
+case: H=>stack [-> H1 H2 H3 H4 H5 H6 H7 H8 H9].
+admit.
+Admitted.
+
